Correct the merge, and simplify the code
TLS 1.2 and 1.3 are working again, using closures to capture connection
state, instead of explicit state structs.

libs/ml/FFI.ml
@@ -1,7 +1,6 @@
+let wrappedConnect12 config host = 
+    TestClient.ffiConnect12 () () () () () () config host
+
 let _ = Callback.register "MITLS_FFI_Config" TestClient13.ffiConfig;
-        Callback.register "MITLS_FFI_Connect12" TestClient13.ffiConnect12;
-        Callback.register "MITLS_FFI_PrepareSend12" TestClient13.ffiPrepareSend12;
-        Callback.register "MITLS_FFI_HandleReceive12" TestClient13.ffiHandleReceive12;
+        Callback.register "MITLS_FFI_Connect12" wrappedConnect12;
         Callback.register "MITLS_FFI_Connect13" TestClient13.ffiConnect13;
-        Callback.register "MITLS_FFI_PrepareSend13" TestClient13.ffiPrepareSend13;
-        Callback.register "MITLS_FFI_HandleReceive13" TestClient13.ffiHandleReceive13;
