src/tls/test/TestClient13.fst
@@ -75,7 +75,6 @@ let recvEncAppDataRecord tcp pv rd =
   IO.print_string ((iutf8 payload)^"\n");
   payload
 
-<<<<<<< HEAD
 // Workaround until KeySchedule is merged in Handshake
 let replace_keyshare ksl e =
   match e with
@@ -84,11 +83,6 @@ let replace_keyshare ksl e =
 
   
 (*****************************************************************************************)
-type ffiStateConfigured = {
-    cscf_guard: string;
-    cscf_config: config;
-    }
-
 let newconfig pv peername =
   if pv = "1.3" then
     let sigPref = [CoreCrypto.RSASIG] in
@@ -101,6 +95,9 @@ let newconfig pv peername =
          maxVer = TLS_1p3;
          ciphersuites = csn;
          peer_name = Some peername;
+         namedGroups = [SEC CoreCrypto.ECC_P256; SEC CoreCrypto.ECC_P384];
+         check_peer_certificate = false;
+         ca_file = "c:\\Repos\\mitls-fstar\\data\\CAFile.pem";
          })
   else
     let l = [ TLS_ECDHE_RSA_WITH_AES_128_GCM_SHA256 ] in
@@ -109,22 +106,17 @@ let newconfig pv peername =
          minVer = TLS_1p2;
          maxVer = TLS_1p2;
          ciphersuites = csn;
+         peer_name = Some peername;
          safe_resumption = true;
          signatureAlgorithms = [(CoreCrypto.RSASIG, Hash CoreCrypto.SHA512); (CoreCrypto.RSASIG, Hash CoreCrypto.SHA384);(CoreCrypto.RSASIG, Hash CoreCrypto.SHA256)];
          check_peer_certificate = false;
-         ca_file = "/cygdrive/c/Repos/mitls/data/CAFile.pem";
-         peer_name = Some peername;
+         ca_file = "c:\\Repos\\mitls-fstar\\data\\CAFile.pem";
          })
-         
-val ffiConfig: string -> string -> ffiStateConfigured  
+
+val ffiConfig: string -> string -> config  
 let ffiConfig tlsversion hostname =
   let config = newconfig tlsversion hostname in
-  let state:ffiStateConfigured =
-  {
-    cscf_guard = "CSCF";
-    cscf_config = config;
-  } in
-  state
+  config
 
     
 (*****************************************************************************************)
@@ -180,61 +172,30 @@ let recvRecordCallback callbacks pv =
 
 let hsbuf = alloc ([] <: list (hs_msg * bytes))
 
-let recvHSRecordCallback12 callbacks pv kex log = 
-  let (hs_msg, to_log) = match !hsbuf with
-    | [] -> 
-      let Correct(ct,rpv,pl) = recvRecordCallback callbacks pv in
-      let hsml = match Handshake.parseHandshakeMessages (Some pv) (Some kex) pl with
-      	         | Correct(_,hsml) -> hsml | Error (y,z) -> IO.print_string(z); failwith "parseHSM failed" in
-      let (hs_msg, to_log)::r = hsml in
-      hsbuf := r; (hs_msg, to_log)
-    | h::t -> hsbuf := t; h in
-  IO.print_string ("Received HS("^(string_of_handshakeMessage hs_msg)^")\n");
-  let logged = handshakeMessageBytes (Some pv) hs_msg in
-  IO.print_string ("Logged message = Parsed message? ");
-  if (Platform.Bytes.equalBytes logged to_log) then IO.print_string "yes\n" else IO.print_string "no\n";
-  (hs_msg,to_log)
-  
-let recvHSRecordCallback callbacks pv kex log = 
+let recvHSRecordCallback callbacks pv kex =
   let Correct(Content.Handshake,rpv,pl) = recvRecordCallback callbacks pv in
   match Handshake.parseHandshakeMessages (Some pv) (Some kex) pl with
   | Correct (rem,[(hs_msg,to_log)]) -> 
      	    (IO.print_string ("Received HS("^(string_of_handshakeMessage hs_msg)^")\n");
-	     (hs_msg,log @| to_log))
+	     (hs_msg, to_log))
   | Error (x,z) -> IO.print_string (z^"\n"); failwith "error"
   
- let recvEncHSRecordCallback callbacks pv kex log rd = 
+ let recvEncHSRecordCallback callbacks pv kex rd = 
   let Correct(Content.Application_data,_,cipher) = recvRecordCallback callbacks pv in
   let payload = decryptRecord_TLS13_AES_GCM_128_SHA256 rd Content.Handshake cipher in
   let Correct (rem,hsm) = Handshake.parseHandshakeMessages (Some pv) (Some kex) payload in 
   let [(hs_msg,to_log)] = hsm in
   IO.print_string ("Received HS("^(string_of_handshakeMessage hs_msg)^")\n");
-  hs_msg, log @| to_log	      
+  hs_msg, to_log	      
   
-let recvEncHSRecordCallback12 callbacks pv kex log rd = 
-  let Correct(Content.Handshake,_,cipher) = recvRecordCallback callbacks pv in
-  let payload = TestClient.decryptRecord_TLS12_AES_GCM_128_SHA256 rd Content.Handshake cipher in
-  let Correct (rem,hsm) = Handshake.parseHandshakeMessages (Some pv) (Some kex) payload in
-  let [(hs_msg,to_log)] = hsm in
-  IO.print_string ("Received HS("^(string_of_handshakeMessage hs_msg)^")\n");
-  let logged = handshakeMessageBytes (Some pv) hs_msg in
-  IO.print_string ("Logged message = Parsed message? ");
-  if (Platform.Bytes.equalBytes logged to_log) then IO.print_string "yes\n" else IO.print_string "no\n";
-  hs_msg,to_log  
-
 let sendRecordCallback callbacks pv ct msg str = 
   let r = Record.makePacket ct pv msg in
   let Correct _ = sendTcpPacket callbacks r in
   IO.print_string ("Sending "^Content.ctToString ct^"Data("^str^")\n")
 
-let sendHSRecordCallback12 callbacks pv (m,b) = 
-  let str = string_of_handshakeMessage m in
-  sendRecordCallback callbacks pv Content.Handshake b str
-
-let sendHSRecordCallback callbacks pv hs_msg log = 
-  let (str,hs,log) = makeHSRecord pv hs_msg log in
-  sendRecordCallback callbacks pv Content.Handshake hs str;
-  log
+let sendHSRecordCallback callbacks pv hs_msg = 
+  let (str,hs) = makeHSRecord pv hs_msg in
+  sendRecordCallback callbacks pv Content.Handshake hs str
     
 let makePacket pv ct msg str = 
   let r = Record.makePacket ct pv msg in
@@ -261,174 +222,45 @@ let check_read header record pv =
          | Error e          -> Error e )
       | Error e             -> Error e )
   | Error e                 -> Error e
+
+  
   
 (*****************************************************************************************)
 
-type ffiStateClient12 = {
-    cscc_guard: string;
-    cscc_pv: protocolVersion;
-    cscc_wr: (StatefulLHAE.writer TestClient.id);
-    cscc_rd: (StatefulLHAE.reader TestClient.id);
-}
-
-let recvCCSRecordCallback callbacks pv = 
-  let Correct(Content.Change_cipher_spec,_,ccs) = recvRecordCallback callbacks pv in
-  IO.print_string "Received CCS\n";
-  ccs
-
-val ffiConnect12: ffiState:ffiStateConfigured -> callbacks:callbacks -> ffiStateClient12
-let ffiConnect12 ffiState callbacks =
-  let _ = (if not (ffiState.cscf_guard = "CSCF") then IO.print_string ("Incorrect cscf_guard "^ffiState.cscf_guard^"\n")) in
-  let config = ffiState.cscf_config in
+let ffiConnect13 config callbacks =
   let rid = new_region root in
-  let log = HandshakeLog.create #rid in
-
-  let ks, cr = KeySchedule.create #rid Client in
-  let (ClientHello ch,chb) = Handshake.prepareClientHello config ks log None None in
-  let pv = ch.ch_protocol_version in 
-  let kex = TLSConstants.Kex_ECDHE in
-
-  sendHSRecordCallback12 callbacks pv (ClientHello ch,chb);
-
-  let (ServerHello(sh),shb) = recvHSRecordCallback12 callbacks pv kex log in
-  
-  let Correct (n,None) = Handshake.processServerHello config ks log None ch (ServerHello(sh),shb) in
-
-  let pv = n.n_protocol_version in
-  let cs = n.n_cipher_suite in
-  let CipherSuite kex sa ae = cs in
-  let ems = n.n_extensions.ne_extended_ms in
-  let sal = n.n_extensions.ne_signature_algorithms in
-
-  let (Certificate(sc),scb) = recvHSRecordCallback12 callbacks pv kex log in
-  IO.print_string ("Certificate validation status = " ^
-    (if Cert.validate_chain sc.crt_chain true config.peer_name config.ca_file then
-      "OK" else "FAIL")^"\n");
-
-  let (ServerKeyExchange(ske),skeb) = recvHSRecordCallback12 callbacks pv kex log in
-  let (ServerHelloDone,shdb) = recvHSRecordCallback12 callbacks pv kex log in
-
-  let tbs = kex_s_to_bytes ske.ske_kex_s in
-  let sigv = ske.ske_sig in
-  let cr = ch.ch_client_random in
-  let sr = sh.sh_server_random in
-  let (ClientKeyExchange cke,ckeb) = 
-     match
-       Handshake.processServerHelloDone config n ks log
-      	[(Certificate sc,scb);(ServerKeyExchange ske, skeb);(ServerHelloDone,shdb)]
-	[] with
-     | Correct [x] -> x 
-     | Error (y,z) -> failwith (z ^ "\n") in
-
-  sendHSRecordCallback12 callbacks pv (ClientKeyExchange cke,ckeb);
-
-  let lb = HandshakeLog.getBytes log in
-  if ems then IO.print_string " ***** USING EXTENDED MASTER SECRET ***** \n";
-//  IO.print_string ("master secret:"^(Platform.Bytes.print_bytes ms)^"\n");
-  let (ck, civ, sk, siv) = KeySchedule.ks_12_get_keys ks in
-  IO.print_string ("client AES_GCM write key:"^(Platform.Bytes.print_bytes ck)^"\n");
-  IO.print_string ("client AES_GCM salt: iv:"^(Platform.Bytes.print_bytes civ)^"\n");
-  IO.print_string ("server AES_GCM write key:"^(Platform.Bytes.print_bytes sk)^"\n");
-  IO.print_string ("server AES_GCM salt:"^(Platform.Bytes.print_bytes siv)^"\n");
-  let wr = TestClient.encryptor_TLS12_AES_GCM_128_SHA256 ck civ in
-  let rd = TestClient.decryptor_TLS12_AES_GCM_128_SHA256 sk siv in
-
-  let (Finished cfin, cfinb) = Handshake.prepareClientFinished ks log in
-  let str = string_of_handshakeMessage (Finished cfin) in 
-  let efinb = TestClient.encryptRecord_TLS12_AES_GCM_128_SHA256 wr Content.Handshake cfinb in
-
-  sendRecordCallback callbacks pv Content.Change_cipher_spec HandshakeMessages.ccsBytes "Client";
-  sendRecordCallback callbacks pv Content.Handshake efinb str;
-
-  let _ = recvCCSRecordCallback callbacks pv in
-  let (Finished(sfin),sfinb) = recvEncHSRecordCallback12 callbacks pv kex log rd in
-  let Correct svd = Handshake.processServerFinished ks log (Finished sfin, sfinb) in
-
-
-  IO.print_string ("Recd fin = expected fin? ");
-  if (Platform.Bytes.equalBytes sfin.fin_vd svd) then IO.print_string "yes\n" else IO.print_string "no\n";
-  let newstate:ffiStateClient12 = {
-    cscc_guard="CSCC";
-    cscc_pv=pv;
-    cscc_wr = wr;
-    cscc_rd = rd;
-  } in
-  newstate
-
-  
-val ffiPrepareSend12:  ffiState:ffiStateClient12 -> cbytes -> cbytes
-let ffiPrepareSend12 ffiState payload =
-  let _ = (if not (ffiState.cscc_guard = "CSHS") then IO.print_string ("Incorrect cscc_guard "^ffiState.cscc_guard^"\n")) in
-  let _ = (if not (ffiState.cscc_pv = TLS_1p2) then IO.print_string ("This call is for TLS 1.2 only\n")) in
-  let pv = ffiState.cscc_pv in
-  let wr = ffiState.cscc_wr in
-  let msg = TestClient.encryptRecord_TLS12_AES_GCM_128_SHA256 wr Content.Application_data (utf8 payload) in
-  let r = makePacket pv Content.Application_data msg "Send" in
-  get_cbytes r
-   
-val ffiHandleReceiveWorker12: ffiState:ffiStateClient12 -> header:bytes -> record:bytes -> (result (bytes))
-let ffiHandleReceiveWorker12 ffiState header record =
-  let _ = (if not (ffiState.cscc_guard = "CSCC") then IO.print_string ("Incorrect cscc_guard "^ffiState.cscc_guard^"\n")) in
-  let _ = (if not (ffiState.cscc_pv = TLS_1p2) then IO.print_string ("This call is for TLS 1.2 only\n")) in
-  let pv = ffiState.cscc_pv in
-  let rd = ffiState.cscc_rd in
-  let c = check_read header record pv in
-  match c with
-  | Error (x,z) -> IO.print_string (z^"\n"); Error (x,z)
-  | Correct(Content.Application_data,_,cipher) -> 
-      let cleartext = TestClient.decryptRecord_TLS12_AES_GCM_128_SHA256 rd Content.Application_data cipher in
-      Correct (cleartext)
-      
-  
-val ffiHandleReceive12:  ffiState:ffiStateClient12 -> header:cbytes -> record:cbytes -> cbytes
-let ffiHandleReceive12 ffiState header record =
-  let h = abytes header in
-  let r = abytes record in
-  match ffiHandleReceiveWorker12 ffiState h r with
-  | Error (x,z) -> IO.print_string (z^"\n"); failwith "error"
-  | Correct (x) -> get_cbytes x 
-  
-(*****************************************************************************************)
-
-type ffiStateClient13 = {
-    cscl_guard: string;
-    cscl_pv: protocolVersion;
-    cscl_dwr: (StreamAE.writer TestClient.id);
-    cscl_drd: (StreamAE.reader TestClient.id);
-}
-  
-val ffiConnect13: ffiState:ffiStateConfigured -> callbacks:callbacks -> ffiStateClient13
-let ffiConnect13 ffiState callbacks =
-  let _ = (if not (ffiState.cscf_guard = "CSCF") then IO.print_string ("Incorrect cscf_guard "^ffiState.cscf_guard^"\n")) in
-  let config = ffiState.cscf_config in
-  let log = empty_bytes in
-  let rid = new_region root in
-  let ks, cr = KeySchedule.create #rid Client in
   let lg = HandshakeLog.create #rid in
+  let ks, cr = KeySchedule.create #rid Client lg in
 
   // This will call KS.ks_client_13_init_1rtt
   let (ClientHello ch,chb) = Handshake.prepareClientHello config ks lg None None in
   let pv = ch.ch_protocol_version in
   let hash x = CoreCrypto.hash CoreCrypto.SHA256 x in
   let kex = TLSConstants.Kex_ECDHE in
-  let log = sendHSRecordCallback callbacks pv (ClientHello ch) log in
+  sendHSRecordCallback callbacks pv (ClientHello ch);
 
-  let ServerHello(sh),log = recvHSRecordCallback callbacks pv kex log in
-  let Correct (n,Some k) = Handshake.processServerHello config ks lg None ch (ServerHello sh,log) in
+  let ServerHello(sh), shb = recvHSRecordCallback callbacks pv kex in
+  
+  let Correct (n,Some k) = Handshake.processServerHello config ks lg None ch (ServerHello sh, shb) in
   let pv = sh.sh_protocol_version in
   let cs = sh.sh_cipher_suite in
-  let CipherSuite kex sa ae = cs in
+  let CipherSuite kex sa (AEAD ae h) = cs in
   let KeySchedule.StAEInstance rd wr = k in
-
   let sal = n.n_extensions.ne_signature_algorithms in
-  let EncryptedExtensions(ee),log = recvEncHSRecordCallback callbacks pv kex log rd in
-  let Certificate(sc),log = recvEncHSRecordCallback callbacks pv kex log rd in
+  
+  let EncryptedExtensions(ee),_ = recvEncHSRecordCallback callbacks pv kex rd in
+  let _ = lg @@ (EncryptedExtensions (ee)) in
+  
+  let Certificate(sc),log = recvEncHSRecordCallback callbacks pv kex rd in
+  let _ = lg @@ Certificate(sc) in
+  
   IO.print_string ("Certificate validation status = " ^
     (if Cert.validate_chain sc.crt_chain true (config.peer_name) config.ca_file then
       "OK" else "FAIL")^"\n");
-  let cv_log = hash log in
+  let cv_log = HandshakeLog.getHash lg h in
 
-  let CertificateVerify(cv),log = recvEncHSRecordCallback callbacks pv kex log rd in
+  let CertificateVerify(cv),log = recvEncHSRecordCallback callbacks pv kex rd in
+  let _ = lg @@ CertificateVerify(cv) in  
 
   //let _ = IO.debug_print_string("cv_sig = " ^ (Platform.Bytes.print_bytes cv.cv_sig) ^ "\n") in
   let Some ((sa,h), sigv) = Handshake.sigHashAlg_of_ske cv.cv_sig in
@@ -439,61 +271,47 @@ let ffiConnect13 ffiState callbacks =
   IO.print_string ("Signature validation status = " ^
     (if Signature.verify h pk tbs sigv then "OK" else "FAIL") ^ "\n");
 
-  let svd = KeySchedule.ks_client_13_1rtt_server_finished ks (hash log) in
-  let Finished({fin_vd = sfin}),log = recvEncHSRecordCallback callbacks pv kex log rd in
+  let svd = KeySchedule.ks_client_13_server_finished ks in
+  let Finished({fin_vd = sfin}),_= recvEncHSRecordCallback callbacks pv kex rd in
+  let _ = lg @@ Finished({fin_vd = sfin}) in
 
   (if equalBytes sfin svd then
     IO.print_string ("Server finished OK:"^(print_bytes svd)^"\n")
   else
     failwith "Failed to verify server finished");
+  (* let KeySchedule.StAEInstance drd dwr = KeySchedule.ks_client_13_sf ks in *)
+  let bb = KeySchedule.ks_client_13_sf ks in
+  let KeySchedule.StAEInstance drd dwr = bb in
 
-  let cvd, (KeySchedule.StAEInstance drd dwr) = KeySchedule.ks_client_13_1rtt_client_finished ks (hash log) in
+  let cvd = KeySchedule.ks_client_13_client_finished ks in
   let cfin = {fin_vd = cvd} in
-  let (str,cfinb,log) = makeHSRecord pv (Finished cfin) log in
+  let (str,cfinb) = makeHSRecord pv (Finished cfin) in
+  let _ = lg @@ (Finished cfin) in
+  
   IO.print_string "before encrypt \n";
   let efinb = encryptRecord_TLS13_AES_GCM_128_SHA256 wr Content.Handshake cfinb in
   sendRecordCallback callbacks pv Content.Application_data efinb str;
-  let newstate:ffiStateClient13 = {
-    cscl_guard="CSCL";
-    cscl_pv=pv;
-    cscl_dwr = dwr;
-    cscl_drd = drd;
-  } in
-  newstate
 
-
-val ffiPrepareSend13:  ffiState:ffiStateClient13 -> cbytes -> cbytes
-let ffiPrepareSend13 ffiState payload =
-  let _ = (if not (ffiState.cscl_guard = "CSCL") then IO.print_string ("Incorrect cscl_guard "^ffiState.cscl_guard^"\n")) in
-  let _ = (if not (ffiState.cscl_pv = TLS_1p3) then IO.print_string ("This call is for TLS 1.3 only\n")) in
-  let pv = ffiState.cscl_pv in
-  let dwr = ffiState.cscl_dwr in
-  let msg = encryptRecord_TLS13_AES_GCM_128_SHA256 dwr Content.Application_data (utf8 payload) in
-  let r = makePacket pv Content.Application_data msg "Send" in
-  get_cbytes r
-
-  
-val ffiHandleReceiveWorker13: ffiState:ffiStateClient13 -> header:bytes -> record:bytes -> (result (bytes))
-let ffiHandleReceiveWorker13 ffiState header record =
-  let _ = (if not (ffiState.cscl_guard = "CSCL") then IO.print_string ("Incorrect cscl_guard "^ffiState.cscl_guard^"\n")) in
-  let _ = (if not (ffiState.cscl_pv = TLS_1p3) then IO.print_string ("This call is for TLS 1.3 only\n")) in
-  let pv = ffiState.cscl_pv in
-  let drd = ffiState.cscl_drd in
-  let c = check_read header record pv in
-  match c with
-  | Error (x,z) -> IO.print_string (z^"\n"); Error (x,z)
-  | Correct(Content.Application_data,_,cipher) -> 
-      let cleartext = decryptRecord_TLS13_AES_GCM_128_SHA256 drd Content.Application_data cipher in
-      Correct (cleartext)
-  
-val ffiHandleReceive13:  ffiState:ffiStateClient13 -> header:cbytes -> record:cbytes -> cbytes
-let ffiHandleReceive13 ffiState header record =
-  let h = abytes header in
-  let r = abytes record in
-  match ffiHandleReceiveWorker13 ffiState h r with
-  | Error (x,z) -> IO.print_string (z^"\n"); failwith "error"
-  | Correct (x) -> get_cbytes x 
-  
+  (* create a closure which is callable as follows:
+      sendrecv(0, packet, _)    <- prepare a packet to send, return is encrypted packet ready to send.
+      sendrecv(1, header, record) <- decrypt a received packet, return is plaintext 
+  *)      
+  let sendrecv what v1 v2 = (
+  IO.print_string ("sendrecv " ^ string_of_int what ^ "\n");
+  match what with
+  | 0 -> (
+    let payload = v1 in
+    let msg = encryptRecord_TLS13_AES_GCM_128_SHA256 dwr Content.Application_data (utf8 payload) in
+    let r = makePacket pv Content.Application_data msg "Send" in
+    get_cbytes r)
+  | 1 -> (
+    let aheader = abytes v1 in
+    let arecord = abytes v2 in
+    let Correct(Content.Application_data,_,cipher) = check_read aheader arecord pv in
+    let p = decryptRecord_TLS13_AES_GCM_128_SHA256 drd Content.Application_data cipher in
+    get_cbytes p)
+  ) in
+  sendrecv
 
   
 let main config host port =
